fix bn_add_mod_n

code/experimental/rsapss/Hacl.Spec.Bignum.fst
@@ -18,9 +18,38 @@ let bn_add_mod_n #len n a b =
   let c0, res0 = bn_add a b in
   let c1, res1 = bn_sub res0 n in
   let c = c0 -. c1 in
-  map2 (mask_select c) res1 res0
+  map2 (mask_select c) res0 res1
 
-let bn_add_mod_n_lemma #len n a b = admit()
+let bn_add_mod_n_lemma #len n a b =
+  let c0, res0 = bn_add a b in
+  bn_add_lemma a b;
+  let c1, res1 = bn_sub res0 n in
+  bn_sub_lemma res0 n;
+  assert (bn_v res1 - v c1 * pow2 (64 * len) == bn_v a + bn_v b - v c0 * pow2 (64 * len) - bn_v n);
+  Math.Lemmas.distributivity_sub_left (v c0) (v c1) (pow2 (64 * len));
+  assert (bn_v res1 + (v c0 - v c1) * pow2 (64 * len) == bn_v a + bn_v b - bn_v n);
+  let c = c0 -. c1 in
+  let res = map2 (mask_select c) res0 res1 in
+
+  if bn_v a + bn_v b < bn_v n then begin
+    assert (v c0 == 0);
+    assert (v c1 == 1);
+    assert (v c == pow2 64 - 1);
+    bn_mask_select_lemma res0 res1 c;
+    assert (bn_v res == bn_v res0);
+    Math.Lemmas.small_mod (bn_v a + bn_v b) (bn_v n);
+    assert (bn_v res == (bn_v a + bn_v b) % bn_v n) end
+  else begin
+    assert (bn_v a + bn_v b - bn_v n < bn_v n);
+    bn_eval_bound res1 len;
+    bn_eval_bound n len;
+    assert (v c == 0);
+    bn_mask_select_lemma res0 res1 c;
+    assert (bn_v res == bn_v res1);
+    Math.Lemmas.modulo_addition_lemma (bn_v a + bn_v b) (bn_v n) (- 1);
+    assert (bn_v res % bn_v n == (bn_v a + bn_v b) % bn_v n);
+    Math.Lemmas.small_mod (bn_v res) (bn_v n) end
+
 
 let bn_mul #aLen #bLen a b =
   Hacl.Spec.Bignum.Multiplication.bn_mul a b
